Updated contract for mem_read, still need to update femtokernel accordingly

case_study/RiscvPmp/BlockVer/Spec.v
@@ -28,7 +28,8 @@
 
 From Coq Require Import
      ZArith.ZArith
-     Strings.String.
+     Strings.String
+     Lists.List.
 From Equations Require Import
      Equations.
 From Katamaran Require Import
@@ -44,9 +45,11 @@ From Katamaran Require Import
      RiscvPmp.IrisModel
      RiscvPmp.IrisInstance
      RiscvPmp.Machine
-     RiscvPmp.Sig.
+     RiscvPmp.Sig
+     RiscvPmp.Contracts.
 
 Import RiscvPmpProgram.
+Import ListNotations.
 
 Set Implicit Arguments.
 Import ctx.resolution.
@@ -87,6 +90,10 @@ Module RiscvPmpBlockVerifSpec <: Specification RiscvPmpBase RiscvPmpProgram Risc
   Notation "a ||ₜ b" := (term_binop bop.or a b) (at level 85).
   Notation asn_match_option T opt xl alt_inl alt_inr := (asn.match_sum T ty.unit opt xl alt_inl "_" alt_inr).
   Notation asn_pmp_entries l := (asn.chunk (chunk_user pmp_entries [l])).
+  Notation asn_pmp_cfg_unlocked e := (asn.formula (formula_user pmp_cfg_unlocked [e])).
+  Notation asn_pmp_all_entries_unlocked l := (asn.chunk (chunk_user pmp_all_entries_unlocked [l])).
+  Notation asn_pmp_addr_access l m := (asn.chunk (chunk_user pmp_addr_access [l; m])).
+  Notation asn_pmp_access addr es m p := (asn.formula (formula_user pmp_access [addr;es;m;p])).
 
   Definition term_eqb {Σ} (e1 e2 : Term Σ ty_regno) : Term Σ ty.bool :=
     term_binop bop.eq e1 e2.
@@ -141,12 +148,14 @@ Module RiscvPmpBlockVerifSpec <: Specification RiscvPmpBase RiscvPmpProgram Risc
 
   (* TODO: abstract away the concrete type, look into unions for that *)
   (* TODO: length of list should be 16, no duplicates *)
-  Definition pmp_entries {Σ} : Term Σ (ty.list (ty.prod ty_pmpcfgidx ty_pmpaddridx)) :=
+  (* Definition pmp_entries {Σ} : Term Σ (ty.list (ty.prod ty_pmpcfgidx ty_pmpaddridx)) :=
     term_list
       (cons (term_val ty_pmpcfgidx PMP0CFG ,ₜ term_val ty_pmpaddridx PMPADDR0)
-            (cons (term_val ty_pmpcfgidx PMP1CFG ,ₜ term_val ty_pmpaddridx PMPADDR1) nil)).
+            (cons (term_val ty_pmpcfgidx PMP1CFG ,ₜ term_val ty_pmpaddridx PMPADDR1) nil)). *)
 
   End ContractDefKit.
+
+  Import RiscvPmpSpecification.
 
   Import asn.notations.
   (* TODO: This notation is already defined with a different meaning in
@@ -162,7 +171,13 @@ Module RiscvPmpBlockVerifSpec <: Specification RiscvPmpBase RiscvPmpProgram Risc
   Local Notation "a ||ₜ b" := (term_binop bop.or a b) (at level 85).
   Local Notation asn_match_option T opt xl alt_inl alt_inr := (asn.match_sum T ty.unit opt xl alt_inl "_" alt_inr).
   Local Notation asn_pmp_entries l := (asn.chunk (chunk_user pmp_entries [l])).
+  Local Notation asn_pmp_cfg_unlocked e := (asn.formula (formula_user pmp_cfg_unlocked [e])).
+  Local Notation asn_pmp_all_entries_unlocked l := (asn.chunk (chunk_user pmp_all_entries_unlocked [l])).
+  Local Notation asn_pmp_addr_access l m := (asn.chunk (chunk_user pmp_addr_access [l; m])).
+  Local Notation asn_pmp_access addr es m p := (asn.formula (formula_user pmp_access [addr;es;m;p])).
   Local Notation "e1 ',ₜ' e2" := (term_binop bop.pair e1 e2) (at level 100).
+  (* TODO: clean up above notations to get rid of the following one *)
+  Local Notation asn_cur_privilege val := (asn.chunk (chunk_ptsreg cur_privilege val)).
   Import bv.notations.
 
 
@@ -210,14 +225,107 @@ Module RiscvPmpBlockVerifSpec <: Specification RiscvPmpBase RiscvPmpProgram Risc
             asn.chunk (chunk_user encodes_instr [term_var "w"; term_var "i"]));
     |}.
 
+  Definition sep_contract_pmpLocked : SepContractFun pmpLocked :=
+    {| sep_contract_logic_variables := ["entry" :: ty_pmpcfg_ent];
+       sep_contract_localstore      := [term_var "entry"];
+       sep_contract_precondition    := asn_pmp_cfg_unlocked (term_var "entry");
+       sep_contract_result          := "result_pmpLocked";
+       sep_contract_postcondition   := term_var "result_pmpLocked" = term_val ty.bool false;
+    |}.
+
+  Definition sep_contract_checked_mem_read : SepContractFun checked_mem_read :=
+    {| sep_contract_logic_variables := ["t" :: ty_access_type; "paddr" :: ty_xlenbits; "p" :: ty_privilege; "entries" :: ty.list ty_pmpentry];
+       sep_contract_localstore      := [term_var "t"; term_var "paddr"];
+       sep_contract_precondition    :=
+           term_var "t" = term_union access_type KRead (term_val ty.unit tt)
+           ∗ term_val ty_xlenbits minAddr <= term_var "paddr"
+           ∗ term_var "paddr" <= term_val ty_xlenbits maxAddr
+           ∗ asn_cur_privilege (term_var "p")
+           ∗ asn_pmp_entries (term_var "entries")
+           ∗ asn_pmp_addr_access (term_var "entries") (term_var "p")
+           ∗ asn_pmp_access (term_var "paddr") (term_var "entries") (term_var "p") (term_var "t");
+       sep_contract_result          := "result_checked_mem_read";
+       sep_contract_postcondition   :=
+         asn_cur_privilege (term_var "p")
+         ∗ asn_pmp_entries (term_var "entries")
+         ∗ asn_pmp_addr_access (term_var "entries") (term_var "p")
+         ∗ asn.exist "v" _ (term_var "result_checked_mem_read" = term_union memory_op_result KMemValue (term_var "v"))
+    |}.
+
+  Definition sep_contract_pmpCheckPerms : SepContractFun pmpCheckPerms :=
+    {| sep_contract_logic_variables := ["entry" :: ty_pmpcfg_ent; "acc" :: ty_access_type; "priv" :: ty_privilege];
+       sep_contract_localstore      := [term_var "entry"; term_var "acc"; term_var "priv"];
+       sep_contract_precondition    :=
+         term_var "priv" = term_val ty_privilege Machine
+         ∗ asn_pmp_cfg_unlocked (term_var "entry");
+       sep_contract_result          := "result_pmpCheckPerms";
+       sep_contract_postcondition   := 
+         term_var "result_pmpCheckPerms" = term_val ty.bool true;
+    |}.
+
+  Definition sep_contract_pmpMatchAddr : SepContractFun pmpMatchAddr :=
+    {| sep_contract_logic_variables := ["addr" :: ty_xlenbits; "rng" :: ty_pmp_addr_range];
+       sep_contract_localstore      := [term_var "addr"; term_var "rng"];
+       sep_contract_precondition    := ⊤;
+       sep_contract_result          := "result_pmpMatchAddr";
+       sep_contract_postcondition   :=
+         term_var "result_pmpMatchAddr" = term_val ty_pmpaddrmatch PMP_NoMatch
+         ∨ term_var "result_pmpMatchAddr" = term_val ty_pmpaddrmatch PMP_Match;
+    |}.
+
+  Definition sep_contract_pmpCheck : SepContractFun pmpCheck :=
+    {| sep_contract_logic_variables := ["addr" :: ty_xlenbits; "acc" :: ty_access_type; "priv" :: ty_privilege; "entries" :: ty.list ty_pmpentry];
+       sep_contract_localstore      := [term_var "addr"; term_var "acc"; term_var "priv"];
+       sep_contract_precondition    :=
+         asn_pmp_entries (term_var "entries")
+         ∗ term_var "priv" = term_val ty_privilege Machine
+         ∗ asn_pmp_all_entries_unlocked (term_var "entries");
+       sep_contract_result          := "result_pmpCheck";
+       sep_contract_postcondition   := 
+         term_var "result_pmpCheck" = term_inr (term_val ty.unit tt)
+         ∗ asn_pmp_entries (term_var "entries")
+         ∗ asn_pmp_access (term_var "addr") (term_var "entries") (term_var "priv") (term_var "acc");
+    |}.
+
+  Definition sep_contract_pmp_mem_read : SepContractFun pmp_mem_read :=
+    {| sep_contract_logic_variables := ["t" :: ty_access_type; "p" :: ty_privilege; "paddr" :: ty_xlenbits; "entries" :: ty.list ty_pmpentry];
+       sep_contract_localstore      := [term_var "t"; term_var "p"; term_var "paddr"];
+       sep_contract_precondition    :=
+           term_var "t" = term_union access_type KRead (term_val ty.unit tt)
+         ∗ term_val ty_xlenbits minAddr <= term_var "paddr"
+         ∗ term_var "paddr" <= term_val ty_xlenbits maxAddr
+         ∗ asn_cur_privilege (term_var "p")
+         ∗ term_var "p" = term_val ty_privilege Machine
+         ∗ asn_pmp_entries (term_var "entries")
+         ∗ asn_pmp_all_entries_unlocked (term_var "entries")
+         ∗ asn_pmp_addr_access (term_var "entries") (term_var "p");
+       sep_contract_result          := "result_pmp_mem_read";
+       sep_contract_postcondition   :=
+         asn_cur_privilege (term_var "p")
+         ∗ asn.exist "v" _ (term_var "result_pmp_mem_read" = term_union memory_op_result KMemValue (term_var "v"))
+         ∗ asn_pmp_entries (term_var "entries")
+         ∗ asn_pmp_addr_access (term_var "entries") (term_var "p");
+    |}.
+
   Definition sep_contract_mem_read : SepContractFun mem_read :=
-    {| sep_contract_logic_variables := ["inv" :: ty.bool; "typ" :: ty_access_type; "paddr" :: ty_xlenbits; "w" :: ty_xlenbits];
+    (* {| sep_contract_logic_variables := ["inv" :: ty.bool; "typ" :: ty_access_type; "paddr" :: ty_xlenbits; "w" :: ty_xlenbits; "entries" :: ty.list ty_pmpentry; "m" :: ty_privilege]; *)
+    {| sep_contract_logic_variables := ["typ" :: ty_access_type; "paddr" :: ty_xlenbits; "entries" :: ty.list ty_pmpentry; "m" :: ty_privilege];
        sep_contract_localstore      := [term_var "typ"; term_var "paddr"];
-       sep_contract_precondition    := asn.match_bool (term_var "inv") (term_var "paddr" ↦ᵣ term_var "w") (term_var "paddr" ↦ₘ term_var "w");
+       sep_contract_precondition    :=
+          term_var "typ" = term_union access_type KRead (term_val ty.unit tt) ∗
+          term_val ty_xlenbits minAddr <= term_var "paddr" ∗
+          term_var "paddr" <= term_val ty_xlenbits maxAddr ∗
+          asn_cur_privilege (term_var "m") ∗
+          term_var "m" = term_val ty_privilege Machine ∗
+          asn_pmp_entries (term_var "entries") ∗
+          asn_pmp_all_entries_unlocked (term_var "entries") ∗
+          asn_pmp_addr_access (term_var "entries") (term_var "m");
+          (* asn.match_bool (term_var "inv") (term_var "paddr" ↦ᵣ term_var "w") (term_var "paddr" ↦ₘ term_var "w"); *)
        sep_contract_result          := "result_mem_read";
        sep_contract_postcondition   :=
-      term_var "result_mem_read" = term_union memory_op_result KMemValue (term_var "w") ∗
-                                     asn.match_bool (term_var "inv") (term_var "paddr" ↦ᵣ term_var "w") (term_var "paddr" ↦ₘ term_var "w");
+         asn.exist "w" ty_xlenbits
+         (term_var "result_mem_read" = term_union memory_op_result KMemValue (term_var "w"));
+                                     (* asn.match_bool (term_var "inv") (term_var "paddr" ↦ᵣ term_var "w") (term_var "paddr" ↦ₘ term_var "w"); *)
     |}.
 
   Definition sep_contract_tick_pc : SepContractFun tick_pc :=
@@ -234,12 +342,19 @@ Module RiscvPmpBlockVerifSpec <: Specification RiscvPmpBase RiscvPmpProgram Risc
   Definition CEnv : SepContractEnv :=
     fun Δ τ f =>
       match f with
-      | rX                    => Some sep_contract_rX
-      | wX                    => Some sep_contract_wX
-      | fetch                 => Some sep_contract_fetch_instr
-      | mem_read              => Some sep_contract_mem_read
-      | tick_pc               => Some sep_contract_tick_pc
-      | _                     => None
+      | rX               => Some sep_contract_rX
+      | wX               => Some sep_contract_wX
+      | fetch            => Some sep_contract_fetch_instr
+      | mem_read         => Some sep_contract_mem_read
+      | tick_pc          => Some sep_contract_tick_pc
+      | pmpCheck         => Some sep_contract_pmpCheck
+      | pmpCheckPerms    => Some sep_contract_pmpCheckPerms
+      | within_phys_mem  => Some sep_contract_within_phys_mem
+      | pmpLocked        => Some sep_contract_pmpLocked
+      | pmpMatchAddr     => Some sep_contract_pmpMatchAddr
+      | pmp_mem_read     => Some sep_contract_pmp_mem_read
+      | checked_mem_read => Some sep_contract_checked_mem_read
+      | _                => None
       end.
 
   Lemma linted_cenv :
@@ -307,20 +422,6 @@ Module RiscvPmpBlockVerifSpec <: Specification RiscvPmpBase RiscvPmpProgram Risc
        lemma_postcondition   := ⊤;
     |}.
 
-  Definition lemma_open_pmp_entries : SepLemma open_pmp_entries :=
-    {| lemma_logic_variables := ctx.nil;
-       lemma_patterns        := env.nil;
-       lemma_precondition    := ⊤;
-       lemma_postcondition   := ⊤;
-    |}.
-
-  Definition lemma_close_pmp_entries : SepLemma close_pmp_entries :=
-    {| lemma_logic_variables := ctx.nil;
-       lemma_patterns        := env.nil;
-       lemma_precondition    := ⊤;
-       lemma_postcondition   := ⊤;
-    |}.
-
   Definition lemma_update_pmp_entries : SepLemma update_pmp_entries :=
     {| lemma_logic_variables := ctx.nil;
        lemma_patterns        := env.nil;
@@ -328,30 +429,16 @@ Module RiscvPmpBlockVerifSpec <: Specification RiscvPmpBase RiscvPmpProgram Risc
        lemma_postcondition   := ⊤;
     |}.
 
-  Definition lemma_extract_pmp_ptsto : SepLemma extract_pmp_ptsto :=
-    {| lemma_logic_variables := ["paddr" :: ty_xlenbits];
-       lemma_patterns        := [term_var "paddr"];
-       lemma_precondition    := ⊤;
-       lemma_postcondition   := ⊤;
-    |}.
-
-  Definition lemma_return_pmp_ptsto : SepLemma return_pmp_ptsto :=
-    {| lemma_logic_variables := ["paddr" :: ty_xlenbits];
-       lemma_patterns        := [term_var "paddr"];
-       lemma_precondition    := ⊤;
-       lemma_postcondition   := ⊤;
-    |}.
-
   Definition LEnv : LemmaEnv :=
     fun Δ l =>
       match l with
-      | open_gprs      => lemma_open_gprs
-      | close_gprs     => lemma_close_gprs
-      | open_pmp_entries => lemma_open_pmp_entries
-      | close_pmp_entries => lemma_close_pmp_entries
-      | update_pmp_entries => lemma_update_pmp_entries
-      | extract_pmp_ptsto => lemma_extract_pmp_ptsto
-      | return_pmp_ptsto => lemma_return_pmp_ptsto
+      | open_gprs                          => lemma_open_gprs
+      | close_gprs                         => lemma_close_gprs
+      | open_pmp_entries                   => lemma_machine_unlocked_open_pmp_entries
+      | close_pmp_entries                  => lemma_machine_unlocked_close_pmp_entries
+      | update_pmp_entries                 => lemma_update_pmp_entries
+      | extract_pmp_ptsto                  => lemma_extract_pmp_ptsto
+      | return_pmp_ptsto                   => lemma_return_pmp_ptsto
       end.
 End RiscvPmpBlockVerifSpec.
 
@@ -368,10 +455,16 @@ Module RiscvPmpSpecVerif.
 
   Import ModalNotations.
 
+  Definition ValidContractDebug {Δ τ} (f : Fun Δ τ) : Prop :=
+    match CEnv f with
+    | Some c => ValidContract c (FunDef f)
+    | None => False
+    end.
+
   Definition ValidContract {Δ τ} (f : Fun Δ τ) : Prop :=
     match CEnv f with
     | Some c => ValidContractReflect c (FunDef f)
-    | None => True
+    | None => False
     end.
 
   Lemma valid_execute_rX : ValidContract rX.
@@ -389,20 +482,178 @@ Module RiscvPmpSpecVerif.
   Lemma valid_execute_tick_pc : ValidContract tick_pc.
   Proof. reflexivity. Qed.
 
-  Lemma valid_execute_mem_read : ValidContract mem_read.
-  Proof. Admitted.
+  Ltac symbolic_simpl :=
+    apply validcontract_with_erasure_sound;
+    compute;
+    constructor;
+    cbn.
 
-  Lemma valid_contracts {Δ τ} (f : Fun Δ τ) :
-    ValidContract f.
+  Import RiscvPmpBlockVerifExecutor.
+
+  Definition ValidContractWithFuel {Δ τ} (fuel : nat) (c : SepContract Δ τ) (body : Stm Δ τ) : Prop :=
+    VerificationCondition
+      (postprocess
+         (SHeapSpecM.vcgen default_config fuel c body)).
+
+  Lemma valid_pmpLocked : ValidContractDebug pmpLocked.
   Proof.
-    unfold ValidContract; destruct f; cbn [CEnv]; try exact I.
-    - apply valid_execute_rX.
-    - apply valid_execute_wX.
-    - apply valid_execute_tick_pc.
-    - apply valid_execute_mem_read.
-    - apply valid_execute_fetch.
+    symbolic_simpl;
+      intros;
+      unfold Pmp_cfg_unlocked in H;
+      simpl in H; now subst.
   Qed.
 
+  Lemma valid_checked_mem_read : ValidContractDebug checked_mem_read.
+  Proof.
+    symbolic_simpl.
+    intros.
+    split; intros.
+    now exists Read.
+    split; intuition.
+  Qed.
+
+  Lemma valid_pmp_mem_read : ValidContract pmp_mem_read.
+  Proof. reflexivity. Qed.
+
+  Lemma valid_pmpMatchAddr : ValidContractDebug pmpMatchAddr.
+  Proof.
+    symbolic_simpl.
+    intros.
+    apply Z.ge_le in H1.
+    apply Zle_imp_le_bool in H1; rewrite H1 in H2.
+    apply Z.gt_lt in H0.
+    apply Z.ltb_lt in H0; rewrite H0 in H2.
+    simpl in *; discriminate.
+  Qed.
+
+  Lemma valid_pmpCheckPerms : ValidContract pmpCheckPerms.
+  Proof. reflexivity. Qed.
+
+  (* TODO: a lot of the following lemmas are copied from the Model, they are only used here, so omit them from the Model? *)
+  (* TODO: we will never have a partial match because we are using integers instead of bitvectors, eventually this lemma will make no sense *)
+  Lemma pmp_match_addr_never_partial : forall (a : Xlenbits) (rng : PmpAddrRange),
+      pmp_match_addr a rng = PMP_Match \/ pmp_match_addr a rng = PMP_NoMatch.
+  Proof.
+    intros a [[lo hi]|].
+    - simpl; destruct (hi <? lo)%Z eqn:H; subst; clear H; first now right.
+      destruct (a <? lo)%Z eqn:?; subst; simpl; first now right.
+      destruct (hi <=? a)%Z eqn:?; subst; simpl; first now right.
+      left.
+      rewrite Z.ltb_antisym in Heqb.
+      rewrite Z.leb_antisym in Heqb0.
+      apply Bool.negb_false_iff in Heqb.
+      apply Bool.negb_false_iff in Heqb0.
+      now rewrite Heqb; rewrite Heqb0.
+    - right; reflexivity.
+  Qed.
+
+  Lemma unlocked_bool : forall (cfg : Pmpcfg_ent),
+      Pmp_cfg_unlocked cfg ->
+      match cfg with
+      | {| L := L |} =>
+          L = false
+      end.
+  Proof. intros []; unfold Pmp_cfg_unlocked; auto. Qed.
+
+  Lemma machine_unlocked_check_pmp_access : forall (cfg0 cfg1 : Pmpcfg_ent) (a0 a1 addr : Xlenbits),
+      Pmp_cfg_unlocked cfg0 /\ Pmp_cfg_unlocked cfg1 ->
+      check_pmp_access addr [(cfg0, a0); (cfg1, a1)]%list Machine = (true, None) \/ check_pmp_access addr [(cfg0, a0); (cfg1, a1)]%list Machine = (true, Some PmpRWX).
+  Proof.
+    intros cfg0 cfg1 a0 a1 addr [Hcfg0 Hcfg1].
+    unfold check_pmp_access, pmp_check.
+    unfold pmp_match_entry.
+    destruct (pmp_match_addr_never_partial addr (pmp_addr_range cfg1 a1 a0)) as [-> | ->];
+      destruct (pmp_match_addr_never_partial addr (pmp_addr_range cfg0 a0 0%Z)) as [-> | ->];
+      destruct cfg0, cfg1;
+      try rewrite (unlocked_bool Hcfg0);
+      try rewrite (unlocked_bool Hcfg1);
+      cbn; auto.
+  Qed.
+
+  Lemma machine_unlocked_pmp_access : forall (addr : Val ty_xlenbits) (cfg0 cfg1 : Val ty_pmpcfg_ent) (a0 a1 : Val ty_xlenbits) (acc : Val ty_access_type),
+      Pmp_cfg_unlocked cfg0 /\ Pmp_cfg_unlocked cfg1 ->
+      Pmp_access addr [(cfg0, a0); (cfg1, a1)]%list Machine acc.
+  Proof.
+    intros.
+    unfold Pmp_access, decide_pmp_access.
+    destruct (machine_unlocked_check_pmp_access a0 a1 addr H) as [|].
+    - destruct (check_pmp_access addr _ Machine).
+      now inversion H0.
+    - destruct (check_pmp_access addr _ Machine).
+      inversion H0.
+      unfold decide_access_pmp_perm; destruct acc; auto.
+  Qed.
+
+  (* This holds, it's just incredibly slow =) *)
+  Lemma valid_pmpCheck : ValidContractWithFuel 10 sep_contract_pmpCheck fun_pmpCheck.
+  Proof.
+  (*   compute. *)
+  (*   constructor. *)
+  (*   cbn. *)
+  (*   intros; subst. *)
+  (*   repeat try split; subst; *)
+  (*   apply (machine_unlocked_pmp_access _ _ _ _ (conj H H0)). *)
+  (* Qed. *)
+  Admitted.
+
+  Lemma valid_mem_read : ValidContract mem_read.
+  Proof. reflexivity. Qed.
+
+  Lemma valid_contract_within_phys_mem : ValidContractDebug within_phys_mem.
+  Proof.
+    symbolic_simpl.
+    intros.
+    rewrite Bool.negb_andb in H.
+    apply Bool.orb_prop in H.
+    destruct H;
+      apply Bool.negb_true_iff in H.
+    apply Z.leb_gt in H; auto.
+    apply Z.leb_gt in H; auto.
+  Qed.
+
+  Lemma valid_contract : forall {Δ τ} (f : Fun Δ τ) (c : SepContract Δ τ),
+      RiscvPmpBlockVerifSpec.CEnv f = Some c ->
+      ValidContract f ->
+      Symbolic.ValidContract c (FunDef f).
+  Proof.
+    intros ? ? f c Hcenv Hvc.
+    unfold ValidContract in Hvc.
+    rewrite Hcenv in Hvc.
+    apply Symbolic.validcontract_reflect_sound.
+    apply Hvc.
+  Qed.
+
+  Lemma valid_contract_debug : forall {Δ τ} (f : Fun Δ τ) (c : SepContract Δ τ),
+      CEnv f = Some c ->
+      ValidContractDebug f ->
+      Symbolic.ValidContract c (FunDef f).
+  Proof.
+    intros ? ? f c Hcenv Hvc.
+    unfold ValidContractDebug in Hvc.
+    rewrite Hcenv in Hvc.
+    apply Hvc.
+  Qed.
+
+  Lemma ValidContracts : forall {Δ τ} (f : Fun Δ τ) (c : SepContract Δ τ),
+      CEnv f = Some c ->
+      Symbolic.ValidContract c (FunDef f).
+  Proof.
+    intros.
+    destruct f; try discriminate H.
+    - apply (valid_contract _ H valid_execute_rX).
+    - apply (valid_contract _ H valid_execute_wX).
+    - apply (valid_contract _ H valid_execute_tick_pc).
+    - apply (valid_contract_debug _ H valid_contract_within_phys_mem).
+    - apply (valid_contract _ H valid_mem_read).
+    - apply (valid_contract_debug _ H valid_checked_mem_read).
+    - apply (valid_contract _ H valid_pmp_mem_read).
+    - apply (valid_contract_debug _ H valid_pmpLocked).
+    - (* apply (valid_contract_debug _ H valid_pmpCheck). *) admit.
+    - apply (valid_contract _ H valid_pmpCheckPerms).
+    - apply (valid_contract_debug _ H valid_pmpMatchAddr).
+    - apply (valid_contract _ H valid_execute_fetch).
+  (* Qed. *)
+  Admitted.
 End RiscvPmpSpecVerif.
 
 Module RiscvPmpIrisInstanceWithContracts.
@@ -581,16 +832,107 @@ Module RiscvPmpIrisInstanceWithContracts.
     - apply decode_sound.
   Qed.
 
+  Ltac destruct_syminstance ι :=
+    repeat
+      match type of ι with
+      | Env _ (ctx.snoc _ (MkB ?s _)) =>
+          let id := string_to_ident s in
+          let fr := fresh id in
+          destruct (env.snocView ι) as [ι fr];
+          destruct_syminstance ι
+      | Env _ ctx.nil => destruct (env.nilView ι)
+      | _ => idtac
+      end.
+
+  Lemma machine_unlocked_open_pmp_entries_sound `{sailGS Σ} :
+    ValidLemma RiscvPmpSpecification.lemma_machine_unlocked_open_pmp_entries.
+  Proof.
+    intros ι; destruct_syminstance ι; cbn.
+    iIntros "(Hentries & Hunlocked)".
+    destruct entries; try done.
+    destruct v as [cfg0 addr0].
+    destruct entries; try done.
+    destruct v as [cfg1 addr1].
+    destruct entries; try done.
+    unfold interp_pmp_all_entries_unlocked.
+    iDestruct "Hunlocked" as "[Hcfg0 Hcfg1]".
+    unfold interp_pmp_entries.
+    iDestruct "Hentries" as "(? & ? & ? & ?)".
+    iExists cfg0.
+    iExists addr0.
+    iExists cfg1.
+    iExists addr1.
+    now iFrame.
+  Qed.
+
+  Lemma machine_unlocked_close_pmp_entries_sound `{sailGS Σ} :
+    ValidLemma RiscvPmpSpecification.lemma_machine_unlocked_close_pmp_entries.
+  Proof.
+    intros ι; destruct_syminstance ι; cbn.
+    iIntros "(? & ? & ? & ? & %Hunlocked0 & %Hunlocked1 & _ & _)".
+    iFrame.
+    now iPureIntro.
+  Qed.
+
+  Lemma in_liveAddrs_split : forall (addr : Addr),
+      (minAddr <= addr)%Z ->
+      (addr <= maxAddr)%Z ->
+      exists l1 l2, liveAddrs = l1 ++ ([addr] ++ l2).
+  Proof.
+    intros addr Hmin Hmax.
+    unfold liveAddrs.
+    exists (seqZ minAddr (addr - minAddr)).
+    exists (seqZ (addr + 1) (maxAddr - addr)).
+    transitivity (seqZ minAddr (addr - minAddr) ++ seqZ (addr) (maxAddr - addr + 1)).
+    refine (eq_trans _ (eq_trans (seqZ_app minAddr (addr - minAddr) (maxAddr - addr + 1) _ _) _));
+      do 2 (f_equal; try lia).
+    f_equal; cbn.
+    refine (eq_trans (seqZ_cons _ _ _) _); try lia.
+    do 2 f_equal; lia.
+  Qed.
+
+  Lemma extract_pmp_ptsto_sound `{sailGS Σ} :
+    ValidLemma RiscvPmpSpecification.lemma_extract_pmp_ptsto.
+  Proof.
+    intros ι; destruct_syminstance ι; cbn.
+    rewrite ?Z.leb_le.
+    iIntros "[Hentries [Hmem [[%Hlemin _] [[%Hlemax _] [%Hpmp _]]]]]".
+    iSplitL "Hentries"; try done.
+    unfold interp_pmp_addr_access_without,
+      interp_pmp_addr_access,
+      interp_ptsto,
+      MemVal, Word.
+
+    destruct (in_liveAddrs_split Hlemin Hlemax) as (l1 & l2 & eq).
+    rewrite eq.
+    rewrite big_opL_app big_opL_cons.
+    iDestruct "Hmem" as "[Hmem1 [Hpaddr Hmem2]]".
+    iSplitR "Hpaddr".
+    - iIntros "Hpaddr".
+      iFrame.
+      now iIntros "_".
+    - iApply "Hpaddr".
+      iPureIntro.
+      now exists acc.
+  Qed.
+
+  Lemma return_pmp_ptsto_sound `{sailGS Σ} :
+    ValidLemma RiscvPmpSpecification.lemma_return_pmp_ptsto.
+  Proof.
+    intros ι; destruct_syminstance ι; cbn.
+    iIntros "[Hentries [Hwithout Hptsto]]".
+    iSplitL "Hentries"; first iFrame.
+    unfold interp_pmp_addr_access_without.
+    iApply ("Hwithout" with "Hptsto").
+  Qed.
+
   Lemma lemSemBlockVerif `{sailGS Σ} : LemmaSem.
   Proof.
-    intros Δ [].
-    - intros ι. now iIntros "_".
-    - intros ι. now iIntros "_".
-    - intros ι. now iIntros "_".
-    - intros ι. now iIntros "_".
-    - intros ι. now iIntros "_".
-    - intros ι. now iIntros "_".
-    - intros ι. now iIntros "_".
+    intros Δ []; intros ι; destruct_syminstance ι; try now iIntros "_".
+    - apply machine_unlocked_open_pmp_entries_sound.
+    - apply machine_unlocked_close_pmp_entries_sound.
+    - apply extract_pmp_ptsto_sound.
+    - apply return_pmp_ptsto_sound.
   Qed.
 
   Import RiscvPmpBlockVerifSpec.
@@ -600,9 +942,8 @@ Module RiscvPmpIrisInstanceWithContracts.
   Proof.
     apply (sound foreignSemBlockVerif lemSemBlockVerif).
     intros Γ τ f c Heq.
-    apply shallow_vcgen_soundness, symbolic_vcgen_soundness, validcontract_reflect_sound.
-    generalize (RiscvPmpSpecVerif.valid_contracts f).
-    unfold RiscvPmpSpecVerif.ValidContract. now rewrite Heq.
+    apply shallow_vcgen_soundness, symbolic_vcgen_soundness.
+    apply RiscvPmpSpecVerif.ValidContracts; assumption.
   Qed.
 
 End RiscvPmpIrisInstanceWithContracts.
